\documentclass{ximera}

\input{../../../preamble.tex}

\author{Jim Fowler}
\license{Creative Commons 4.0 By-SA}

\begin{document}

\begin{exercise}
Consider $F(x,y,z) = e^{x+y+z}$ over the region defined by
$$
D = \{ (x,y,z) \in \R^3 : x \geq 0 \mbox{ and } \mbox{ and } y \geq 0
\mbox{ and } z \geq 0 \mbox{ and } x+y+z \leq 1 \}.
$$
to get
\[
  \iiint_D F \d V = \answer{\frac{e}{2} - 1}.
\]

\begin{hint}
This is the integral
$$
I := \int_{x=0}^1 \int_{y=0}^{1-x} \int_{z=0}^{1-x-y} e^{x+y+z} \, dz \, dy \, dx,
$$
\end{hint}
\begin{hint}
We can compute as follows:
\begin{align*}
  I
&= \int_{x=0}^1 \int_{y=0}^{1-x} \int_{z=0}^{1-x-y} e^{x+y+z} \, dz \, dy \, dx \\
&= \int_{x=0}^1 e^x \int_{y=0}^{1-x} e^y \int_{z=0}^{1-x-y} e^z \, dz \, dy \, dx \\
&= \int_{x=0}^1 e^x \int_{y=0}^{1-x} e^y (e^{1-x-y} - 1) \, dy \, dx \\
&= \int_{x=0}^1 e^x (y e^{1-x} - e^y)_{y=0}^{1-x} \, dx \\
&= \int_{x=0}^1 e^x ((1-x) e^{1-x} - e^{1-x} + 1)_{y=0}^{1-x} \, dx \\
&= \int_{x=0}^1 ((1-x) e - e + e^x) \, dx \\
&= \int_{x=0}^1 (-xe + e^x) \, dx \\
&= \left( \frac{-x^2}{2} e + e^x \right)_{x=0}^{1} \\
&= \frac{e}{2} - 1.
\end{align*}
\end{hint}
\end{exercise}
\end{document}