\documentclass{ximera}

\input{../preamble.tex}

	\outcome{Recognize a composition of functions.}
	\outcome{Take derivatives of compositions of functions using the chain rule.}
	\outcome{Take derivatives that require the use of multiple derivative rules.}
	\outcome{Use the chain rule to calculate derivatives from a table of values.}
	\outcome{Understand rate of change when quantities are dependent upon each other.}
	\outcome{Use order of operations in situations requiring multiple derivative rules.}
    \outcome{Justify the chain rule via the composition of linear approximations.}
    \outcome{Apply chain rule to relate quantities expressed with different units.}

\title[Dig-In:]{The chain rule}

\begin{document}
\begin{abstract}
Here we compute derivatives of compositions of functions
\end{abstract}
\maketitle


So far we have seen how to compute the derivative of a function built
up from other functions by addition, subtraction, multiplication and
division. There is another very important way that we combine
functions: composition. The \textit{chain rule} allows us to deal with
this case.


Consider
\[
h(x) = (1+2x)^5.
\] 

While there are several different ways to differentiate this function,
if we let $f(x) = x^5$ and $g(x) = 1+2x$, then we can express $h(x) =
\answer[given]{f}(\answer[given]{g}(x))$. The question is, can we compute the derivative of a
composition of functions using the derivatives of the constituents
$f(x)$ and $g(x)$? To do so, we need the \textit{chain rule}.

\begin{image}
\begin{tikzpicture}
	\begin{axis}[
            axis lines=none,
            clip=false,
          ]          
          \addplot [->,textColor] plot coordinates {(0,0) (-2,-4)}; %% x axis
          \addplot [->,textColor] plot coordinates {(0,0) (0,6)}; %% y axis
          \addplot [->,textColor] plot coordinates {(0,0) (6,0)}; %% g(x) axis

          \addplot [dashed, textColor] plot coordinates {(-.7,-1.4) (1.4,-1.4)};
          \addplot [dashed, textColor] plot coordinates {(1.4,-1.4) (2.1,0)};
          \addplot [dashed, textColor] plot coordinates {(2.1,0) (2.1,4.1)};
          
          \addplot [dashed, textColor] plot coordinates {(2.6,-2.6) (3.5,0)};
          \addplot [dashed, textColor] plot coordinates {(3.5,0) (3.5,4.1)};

          \addplot [dashed, very thick, textColor] plot coordinates {(1.4,-1.4) (.8,-2.6)};
          \addplot [dashed, very thick, textColor] plot coordinates {(2.1,4.1) (3.5,4.1)};

          \addplot [very thick, penColor5] plot coordinates {(.8,-2.6) (2.6,-2.6)};
          \addplot [very thick, penColor4] plot coordinates {(3.5,4.1) (3.5,5.5)};

          \addplot [very thick,penColor,domain=(0:4)] {2+x};
          \addplot [very thick,penColor2,domain=(0:4)] {-x};

          \node at (axis cs:3.5,4.8) [anchor=west,penColor4] {$f'(g(a)){\color{penColor5}g'(a)h}$};
          \node at (axis cs:1.7,-2.6) [anchor=north,penColor5] {$g'(a)h$};
          
          \addplot[color=penColor2,fill=penColor2,only marks,mark=*] coordinates{(1.4,-1.4)};  %% closed hole          
          \addplot[color=penColor,fill=penColor,only marks,mark=*] coordinates{(2.1,4.1)};  %% closed hole          

          \node at (axis cs:1,-2.1) [anchor=south,yslant=0,xslant=0,rotate=53] {$\overbrace{\hspace{.36in}}^{h}$};
          \node at (axis cs:7,0) [anchor=east] {$g(x)$};
          \node at (axis cs:0,6.7) [anchor=north] {$y$};
          \node at (axis cs:-2.15,-4) [anchor=north] {$x$};
          \node at (axis cs:-.7,-1.4) [anchor=east] {$a$};
        \end{axis}
\end{tikzpicture}
%% \caption{A geometric interpretation of the chain rule. Increasing $a$
%%   by a ``small amount'' $h$, increases $f(g(a))$ by $f'(g(a))g'(a)h$. Hence, 
%% \[
%% \frac{\Delta y}{\Delta x}\approx \frac{f'(g(a))g'(a)h}{h} =
%% f'(g(a))g'(a).
%% \]} 
\end{image}
\begin{theorem}[Chain Rule]\index{chain rule}\index{derivative rules!chain}
If $f(x)$ and $g(x)$ are differentiable, then
\[
\ddx f(g(x)) = f'(g(x))g'(x).
\]
\end{theorem}

\begin{proof}
Let $g_0$ be some $x$-value and consider the following:
\[
f'(g_0) = \lim_{h\to 0}\frac{f(g_0+h)-f(g_0)}{h}.
\]

Set $h = g-g_0$ and we have
\begin{equation}\label{E:chainRuleLim}
f'(g_0) = \lim_{g\to g_0} \frac{f(g)-f(g_0)}{g-g_0}.
\end{equation}
At this point, we might like to set $g=g(x+h)$ and $g_0=g(x)$;
however, we cannot as we cannot be sure that
\[
g(x+h) - g(x) \ne 0\qquad\text{when $h\ne 0$.}
\]
To overcome this difficulty, let $E(g)$ be the ``error term'' that
gives the difference between the slope of the secant line from
$f(g_0)$ to $f(g)$ and $f'(g_0)$,
\[
E(g) = \frac{f(g)-f(g_0)}{g-g_0} - f'(g_0).
\]
In particular, $E(g)(g-g_0)$ is the difference between $f(g)$ and the
tangent line of $f(x)$ at $x=g$, see the figure below:

\begin{image}
\begin{tikzpicture}
	\begin{axis}[
            clip=false,
            domain=0:2, range=0:6,ymax=4,ymin=0,
            axis lines =left, xlabel=$x$, ylabel=$y$,
            every axis y label/.style={at=(current axis.above origin),anchor=south},
            every axis x label/.style={at=(current axis.right of origin),anchor=west},
            xtick={1,1.666}, ytick={1,3},
            xticklabels={$g_0$,$g$}, yticklabels={$f(g_0)$,$f(g)$},
            axis on top,
          ]         
	  \addplot [textColor,dashed] plot coordinates {(1,0) (1,1)};
          \addplot [textColor,dashed] plot coordinates {(0,1) (1,1)};
          \addplot [textColor,dashed] plot coordinates {(0,3) (1.666,3)};
          \addplot [textColor,dashed] plot coordinates {(1.666,0) (1.666,1)};

          \addplot [textColor,dashed,very thick] plot coordinates {(1,1) (1.666,1)};
          \node at (axis cs:1.333,1) [anchor=north] {$\underbrace{\hspace{.75in}}_{g-g_0}$};

          \addplot [penColor4,very thick] plot coordinates {(1.666,1) (1.666,1.666)};
          \addplot [penColor5,very thick] plot coordinates {(1.666,1.666) (1.666,3)};

          \node at (axis cs:1.666,1.333) [anchor=west] {$f'(g_0)(g-g_0)$};
          \node at (axis cs:1.666,2.333) [anchor=west] {$E(g)(g-g_0)$};

          \addplot [very thick,penColor, smooth,domain=(0:7/4)] {-1/(x-2)};
          \addplot [very thick,penColor2, smooth,domain=(0:2)] {x};

          \addplot[color=penColor,fill=penColor,only marks,mark=*] coordinates{(1.666,3)};  %% closed hole          
          \addplot[color=penColor,fill=penColor,only marks,mark=*] coordinates{(1,1)};  %% closed hole          
        \end{axis}
\end{tikzpicture}
\end{image}

Hence we see that
\begin{equation}\label{E:chainRuleDer}
f(g)-f(g_0) = \left(f'(g_0) + E(g)\right)(g-g_0),
\end{equation}
and so
\[
\frac{f(g)-f(g_0)}{g-g_0} = f'(g_0) + E(g).
\]


Combining this with Equation~\ref{E:chainRuleLim}, we have that
\begin{align*}
f'(g_0) &= \lim_{g\to g_0}\frac{f(g)-f(g_0)}{g-g_0} \\
&= \lim_{g\to g_0}f'(g_0) + E(g)\\
&= f'(g_0) + \lim_{g\to g_0} E(g),
\end{align*}
and hence it follows that $\lim_{g\to g_0} E(g) = 0$. At this point,
we may return to the ``well-worn path.'' Starting with
Equation~\ref{E:chainRuleDer}, divide both sides by $h$ and set
$g=g(x+h)$ and $g_0=g(x)$
\[
\frac{f(g(x+h))-f(g(x))}{h} = \left(f'(g(x)) +
E(g(x+h))\right)\frac{g(x+h)-g(x)}{h}.
\]
Taking the limit as $h$ approaches $0$, we see 
\begin{align*}
\lim_{h\to 0}\frac{f(g(x+h))-f(g(x))}{h} &= \lim_{h\to 0}\left(f'(g(x))
+ E(g(x+h))\right)\frac{g(x+h)-g(x)}{h}\\
&= \lim_{h\to 0}\left(f'(g(x))
+ E(g(x+h))\right)\lim_{h\to 0}\frac{g(x+h)-g(x)}{h}\\
&= f'(g(x))g'(x).
\end{align*}
Hence, $\ddx f(g(x))= f'(g(x))g'(x)$.
\end{proof}


It will take a bit of practice to make the use of the chain rule come
naturally---it is more complicated than the earlier differentiation
rules we have seen. Let's return to our motivating example.

\begin{example}
Compute:
\[
\ddx (1+2x)^5
\]

\begin{explanation}
Set $f(x) = x^5$ and $g(x) = 1+2x$, now
\[
f'(x) = \answer[given]{5x^4} \qquad\text{and}\qquad g'(x) = \answer[given]{2}.
\]
Hence
\begin{align*}
\ddx (1+2x)^5 &= \ddx f(g(x))\\ 
&=f'(g(x))g'(x) \\
&= 5(\answer[given]{1+2x})^4\cdot \answer[given]{2}\\
&= 10(1+2x)^4.
\end{align*}
\end{explanation}
\end{example}


Let's see a more complicated chain of compositions.

\begin{example}
Compute:
\[
\ddx \sqrt{1+\sqrt{x}}
\]

\begin{explanation}
Set 
$f(x)=\sqrt{x}$ and $g(x)=1+x$. Hence,
\[
\sqrt{1+\sqrt{x}}=f(g(\answer[given]{f}(x))) \qquad\text{and}\qquad\ddx f(g(f(x))) = f'(g(f(x)))g'(f(x))f'(x).
\]
Since 
\[
f'(x) = \answer[given]{\frac{1}{2\sqrt{x}}} \qquad\text{and}\qquad g'(x) = \answer[given]{1}
\]
We have that
\[
\ddx \sqrt{1+\sqrt{x}} = \frac{1}{2\sqrt{1+\sqrt{x}}}\cdot 1\cdot  \answer[given]{\frac{1}{2\sqrt{x}}}.
\]
\end{explanation}
\end{example}

Using the chain rule, the power rule, and the product rule it is
possible to avoid using the quotient rule entirely.

\begin{example}
Compute:
\[
\ddx \frac{x^3}{x^2+1}
\]

\begin{explanation}
Rewriting this as 
\[
\ddx x^3(x^2+1)^{-1}, 
\]
set $f(x) = \answer[given]{x^{-1}}$ and $g(x) = \answer[given]{x^2+1}$ so that $f(g(x)) = (x^2 + 1)^{-1}$. Now
\[
x^3(x^2+1)^{-1} = x^3 f(g(x)) \qquad\text{and}\qquad \ddx x^3 f(g(x)) = \answer[given]{3x^2} \cdot f(g(x))+ \answer[given]{x^3} \cdot f'(g(x))g'(x).
\]
Since $f'(x) = \answer[given]{\frac{-1}{x^2}}$ and $g'(x) = \answer[given]{2x}$, write
\[
\ddx \frac{x^3}{x^2+1} = \frac{3x^2}{x^2+1}-\frac{2x^4}{(x^2+1)^2}.
\]
\end{explanation}
\end{example}

\end{document}
