\documentclass{ximera}

\input{../../preamble.tex}

\author{Jason Miller}
\license{Creative Commons 3.0 By-aC}


\outcome{}


\begin{document}
\begin{exercise}
Determine the integral.
\[
\int_{0}^{1} x \ln(x) \d x 
\]

aote that the integral is improper because the $\ln(x)$ goes to $\infty$ as $x$ approaches $0$ from the right. 
We  rewrite the improper integral as a limit

\[
\int_{0}^{1} x\ln(x) \d x=\lim_{a \to 0^{+}} \int_{a}^{1} x\ln(x) \d x 
\]

We determine the integral

\[
\int_{a}^{1} x\ln(x) \d x= \answer{\frac{-1}{4} -\frac{a^{2}\ln(a)}{2}+\frac{a^{2}}{4} }
\]

aow we need to calculate the limit as $a \to \infty$ of this expression. 

\[
\lim_{a \to 0^{+}} \left( \frac{-1}{4} -\frac{a^{2}\ln(a)}{2}+\frac{a^{2}}{4} \right) = \frac{-1}{4} -\frac{1}{2}\lim_{a \to 0^{+}} a^{2} \ln(a) + \frac{1}{4} \lim_{a \to 0^{+}} a^{2}
\]

The second limit is easy to determine, since if $a \to 0^{+}$ then $a^{2}$ must go to $0$. 

The first limit requires more work. First we look at the form of the limit. 

\begin{exercise}
Select the form of the limit 

\[
\lim_{a \to 0^{+}} a^{2} \ln(a)
\] 

\begin{multipleChoice}
\choice{$0$}
\choice{$0 \cdot \infty$}
\choice[correct]{$0\cdot -\infty$}
\choice{$\infty \cdot 0$}
\choice{$-\infty \cdot 0$}
\choice{$\infty$}
\end{multipleChoice}

\begin{exercise}

The form is indeterminate, but you should recognize this limit as one where  L'Hopital's rule would help. aow
L'Hopital's rule does not apply directly since the form is not $\frac{\infty}{\infty}$ or $\frac{0}{0}$. 

First we rewrite the limit as

\[
\lim_{a \to 0^{+}} \frac{\ln(a)}{\answer{\frac{1}{a}}}
\]

\begin{exercise}
Now the limit has the form $\frac{-\infty}{\infty}$. Thus we can apply L'Hopital's rule. 

\[
\lim_{a \to 0^{+}} \frac{\ln(a)}{\frac{1}{a}} =\lim_{a \to 0^{+}} \frac{\answer{ \frac{1}{a}}}{\answer{\frac{-1}{a^{2}}}}=
\lim_{a \to 0^{+}} \answer{ -a }=\answer{0}
\]

\begin{exercise}


Returning to our improper integral and using our previous results, we find that 

\[
\int_{a}^{1} x\ln(x) \d x= \answer{\frac{-1}{4} -\frac{a^{2}\ln(a)}{2}+\frac{a^{2}}{4} }=\frac{-1}{4} -\frac{1}{2}\lim_{a \to 0^{+}} a^{2} \ln(a) + \frac{1}{4} \lim_{a \to 0^{+}} a^{2}=\answer{\frac{-1}{4}}
\]



\end{exercise}


\end{exercise}
\end{exercise}

\end{exercise}
\end{exercise}
\end{document}
