\documentclass{ximera}

\input{../preamble.tex}

\title[Reinforce:]{Derivative practice}

\begin{document}
\begin{abstract}
  Drills for derivatives.
\end{abstract}
\maketitle


\begin{shuffle}


\begin{exercise}
%% 1
Let $f(x)=-e^{2 x-1} \cos (x)$.
\[
\ddx f(x) = \answer{e^{2 x-1} (\sin (x)-2 \cos (x))}
\]
\end{exercise}

\begin{exercise}
%% 2
Let $f(x)=\frac{2}{x^8}+\sqrt{x}+e^{3 x}+\frac{1}{\sqrt[6]{x}}$.
\[
\ddx f(x) = \answer{\frac{x^{17/2}-32}{2 x^9}+3 e^{3 x}-\frac{1}{6 \sqrt[6]{x}^7}}
\]
\end{exercise}

\begin{exercise}
%% 3
Let $f(x)=\left(x^4-4\right) (x \sec (x)+4)$.
\[
\ddx f(x) = \answer{\left(x^4-4\right) (x \tan (x)+1) \sec (x)+4 x^3 (x \sec (x)+4)}
\]
\end{exercise}

\begin{exercise}
%% 4
Let $f(x)=4 x^{\pi }+4^x+x 4^{\sec (2)}+e^4$.
\[
\ddx f(x) = \answer{4 \pi  x^{\pi -1}+4^x \ln (4)+4^{\sec (2)}}
\]
\end{exercise}

\begin{exercise}
%% 5
Let $f(x)=\tan \left(\frac{x^4-3 x}{3 x^5+3}\right)$.
\[
\ddx f(x) = \answer{-\frac{\left(x^8-12 x^5-4 x^3+3\right) \sec ^2\left(\frac{x \left(x^3-3\right)}{3 \left(x^5+1\right)}\right)}{3 \left(x^5+1\right)^2}}
\]
\end{exercise}

\begin{exercise}
%% 6
Let $f(x)=\frac{\csc ^7(x)+\ln (5)}{\sqrt{x^8+3}-2}$.
\[
\ddx f(x) = \answer{\frac{-7 \left(\sqrt{x^8+3}-2\right) \cot (x) \csc ^7(x)-\frac{4 x^7 \left(\csc ^7(x)+\ln (5)\right)}{\sqrt{x^8+3}}}{\left(\sqrt{x^8+3}-2\right)^2}}
\]
\end{exercise}

\begin{exercise}
%% 7
Let $f(x)=x \ln (x \ln (x))$.
\[
\ddx f(x) = \answer{\ln (x \ln (x))+\frac{1}{\ln (x)}+1}
\]
\end{exercise}

\begin{exercise}
%% 8
Let $f(x)=\sqrt{-\frac{3}{x^6}-2 x}$.
\[
\ddx f(x) = \answer{\frac{9-x^7}{\sqrt{-\frac{3}{x^6}-2 x} x^7}}
\]
\end{exercise}

\begin{exercise}
%% 9
Let $f(x)=4 x^{20}+e^x x+\cos ^6(3)$.
\[
\ddx f(x) = \answer{80 x^{19}+e^x (x+1)}
\]
\end{exercise}

\begin{exercise}
%% 10
Let $f(x)=\frac{117649}{x^{30}}+\frac{3}{\sqrt{x}}+\frac{\cot (x)}{x}$.
\[
\ddx f(x) = \answer{-\frac{3 x^{59/2}+2 x^{30} \csc ^2(x)+2 x^{29} \cot (x)+7058940}{2 x^{31}}}
\]
\end{exercise}

\begin{exercise}
%% 11
Let $f(x)=\sqrt{x} e^{-2 x}-\frac{3 \pi }{x^7}$.
\[
\ddx f(x) = \answer{\frac{e^{-2 x} \left(42 \pi  e^{2 x}-4 x^{17/2} \ln (e)+x^{15/2}\right)}{2 x^8}}
\]
\end{exercise}

\begin{exercise}
%% 12
Let $f(x)=-\frac{2 x}{\ln (x)-2 x^6}$.
\[
\ddx f(x) = \answer{-\frac{2 \left(10 x^6+\ln (x)-1\right)}{\left(\ln (x)-2 x^6\right)^2}}
\]
\end{exercise}

\begin{exercise}
%% 13
Let $f(x)=-e^{\sin (x)} \csc (2 x)$.
\[
\ddx f(x) = \answer{-e^{\sin (x)} \csc (2 x) (\cos (x)-2 \cot (2 x))}
\]
\end{exercise}

\begin{exercise}
%% 14
Let $f(x)=\sqrt{\cos (x)+e^2+3}$.
\[
\ddx f(x) = \answer{-\frac{\sin (x)}{2 \sqrt{\cos (x)+e^2+3}}}
\]
\end{exercise}

\begin{exercise}
%% 15
Let $f(x)=\csc (\ln (x))$.
\[
\ddx f(x) = \answer{-\frac{\cot (\ln (x)) \csc (\ln (x))}{x}}
\]
\end{exercise}

\begin{exercise}
%% 16
Let $f(x)=\ln (\cot (x))$.
\[
\ddx f(x) = \answer{-\csc (x) \sec (x)}
\]
\end{exercise}

\begin{exercise}
%% 1
Let $f(x)=e^{4 x-1} \cos (x)$.
\[
\ddx f(x) = \answer{e^{4 x-1} (4 \cos (x)-\sin (x))}
\]
\end{exercise}

\begin{exercise}
%% 2
Let $f(x)=\frac{3}{x^5}+\sqrt{x}+e^{3 x}+\frac{1}{\sqrt{x}}$.
\[
\ddx f(x) = \answer{\frac{x^{11/2}-x^{9/2}+6 e^{3 x} x^6-30}{2 x^6}}
\]
\end{exercise}

\begin{exercise}
%% 3
Let $f(x)=\left(\frac{1}{x^4}-3\right) (x \csc (x)+2)$.
\[
\ddx f(x) = \answer{\left(\frac{1}{x^4}-3\right) (1-x \cot (x)) \csc (x)-\frac{4 (x \csc (x)+2)}{x^5}}
\]
\end{exercise}

\begin{exercise}
%% 4
Let $f(x)=4 x^{-e}+4^x+x 4^{\sec (2)}+\cos ^4(2)$.
\[
\ddx f(x) = \answer{-4 e x^{-1-e}+4^x \ln (4)+4^{\sec (2)}}
\]
\end{exercise}

\begin{exercise}
%% 5
Let $f(x)=\sin \left(\frac{x^8+4 x}{3-4 x^4}\right)$.
\[
\ddx f(x) = \answer{-\frac{4 \left(4 x^{11}-6 x^7-12 x^4-3\right) \cos \left(\frac{x \left(x^7+4\right)}{3-4 x^4}\right)}{\left(3-4 x^4\right)^2}}
\]
\end{exercise}

\begin{exercise}
%% 6
Let $f(x)=\frac{\sec ^7(x)+\pi }{\sqrt{x^8+4}+3}$.
\[
\ddx f(x) = \answer{\frac{7 \left(\sqrt{x^8+4}+3\right) \tan (x) \sec ^7(x)-\frac{4 x^7 \left(\sec ^7(x)+\pi \right)}{\sqrt{x^8+4}}}{\left(\sqrt{x^8+4}+3\right)^2}}
\]
\end{exercise}

\begin{exercise}
%% 7
Let $f(x)=x \ln (x \ln (x))$.
\[
\ddx f(x) = \answer{\ln (x \ln (x))+\frac{1}{\ln (x)}+1}
\]
\end{exercise}

\begin{exercise}
%% 8
Let $f(x)=\sqrt{3 x-\frac{3}{x^5}}$.
\[
\ddx f(x) = \answer{\frac{\frac{15}{x^6}+3}{2 \sqrt{3 x-\frac{3}{x^5}}}}
\]
\end{exercise}

\begin{exercise}
%% 9
Let $f(x)=2 x^{35}+e^x x+\pi ^5$.
\[
\ddx f(x) = \answer{70 x^{34}+e^x (x+1)}
\]
\end{exercise}

\begin{exercise}
%% 10
Let $f(x)=\frac{16807}{x^{35}}-\frac{2}{\sqrt{x}}+\frac{\cot (x)}{x}$.
\[
\ddx f(x) = \answer{\frac{x^{69/2}+x^{35} \left(-\csc ^2(x)\right)-x^{34} \cot (x)-588245}{x^{36}}}
\]
\end{exercise}

\begin{exercise}
%% 11
Let $f(x)=\sqrt{x} e^{-3 x}+\frac{2 \sec (3)}{x^4}$.
\[
\ddx f(x) = \answer{\frac{e^{-3 x}}{2 \sqrt{x}}-3 \sqrt{x} e^{-3 x} \ln (e)-\frac{8 \sec (3)}{x^5}}
\]
\end{exercise}

\begin{exercise}
%% 12
Let $f(x)=-\frac{4 x}{\ln (x)-4 x^4}$.
\[
\ddx f(x) = \answer{-\frac{4 \left(12 x^4+\ln (x)-1\right)}{\left(\ln (x)-4 x^4\right)^2}}
\]
\end{exercise}

\begin{exercise}
%% 13
Let $f(x)=e^{\tan (x)} \sec (2 x)$.
\[
\ddx f(x) = \answer{e^{\tan (x)} \sec (2 x) \left(2 \tan (2 x)+\sec ^2(x)\right)}
\]
\end{exercise}

\begin{exercise}
%% 14
Let $f(x)=\sqrt{\cos (x)+3+\cos (3)}$.
\[
\ddx f(x) = \answer{-\frac{\sin (x)}{2 \sqrt{\cos (x)+3+\cos (3)}}}
\]
\end{exercise}

\begin{exercise}
%% 15
Let $f(x)=\tan (\ln (x))$.
\[
\ddx f(x) = \answer{\frac{\sec ^2(\ln (x))}{x}}
\]
\end{exercise}

\begin{exercise}
%% 16
Let $f(x)=\ln (\cot (x))$.
\[
\ddx f(x) = \answer{-\csc (x) \sec (x)}
\]
\end{exercise}

\begin{exercise}
%% 1
Let $f(x)=e^{-3 x} \cos (3) \sec (x)$.
\[
\ddx f(x) = \answer{e^{-3 x} \cos (3) (\tan (x)-3) \sec (x)}
\]
\end{exercise}

\begin{exercise}
%% 2
Let $f(x)=-\frac{4}{x^4}+\sqrt{x}+e^{4 x}+\frac{1}{\sqrt{x}}$.
\[
\ddx f(x) = \answer{\frac{x^{9/2}-x^{7/2}+8 e^{4 x} x^5+32}{2 x^5}}
\]
\end{exercise}

\begin{exercise}
%% 3
Let $f(x)=\left(x^7-4\right) (x \cot (x)-4)$.
\[
\ddx f(x) = \answer{\left(x^7-4\right) \left(\cot (x)-x \csc ^2(x)\right)+7 x^6 (x \cot (x)-4)}
\]
\end{exercise}

\begin{exercise}
%% 4
Let $f(x)=5 x^e+5^x+x 5^{\ln (4)}+e^{10}$.
\[
\ddx f(x) = \answer{5 e x^{e-1}+5^x \ln (5)+5^{\ln (4)}}
\]
\end{exercise}

\begin{exercise}
%% 5
Let $f(x)=\cos \left(\frac{x^4-2 x}{4 x^6-4}\right)$.
\[
\ddx f(x) = \answer{\frac{\left(x^9-5 x^6+2 x^3-1\right) \sin \left(\frac{x \left(x^3-2\right)}{4 \left(x^6-1\right)}\right)}{2 \left(x^6-1\right)^2}}
\]
\end{exercise}

\begin{exercise}
%% 6
Let $f(x)=\frac{\sin ^5(x)-e}{\sqrt{x^4+3}-2}$.
\[
\ddx f(x) = \answer{\frac{5 \left(\sqrt{x^4+3}-2\right) \sin ^4(x) \cos (x)+\frac{2 x^3 \left(e-\sin ^5(x)\right)}{\sqrt{x^4+3}}}{\left(\sqrt{x^4+3}-2\right)^2}}
\]
\end{exercise}

\begin{exercise}
%% 7
Let $f(x)=x \ln (x \ln (x))$.
\[
\ddx f(x) = \answer{\ln (x \ln (x))+\frac{1}{\ln (x)}+1}
\]
\end{exercise}

\begin{exercise}
%% 8
Let $f(x)=\sqrt{2 x-\frac{3}{x^8}}$.
\[
\ddx f(x) = \answer{\frac{x^9+12}{x^9 \sqrt{2 x-\frac{3}{x^8}}}}
\]
\end{exercise}

\begin{exercise}
%% 9
Let $f(x)=3 x^{24}+e^x x+\ln ^8(4)$.
\[
\ddx f(x) = \answer{72 x^{23}+e^x (x+1)}
\]
\end{exercise}

\begin{exercise}
%% 10
Let $f(x)=\frac{823543}{x^{56}}-\frac{2}{\sqrt{x}}+\frac{\csc (x)}{x}$.
\[
\ddx f(x) = \answer{\frac{x^{111/2}-x^{55} (x \cot (x)+1) \csc (x)-46118408}{x^{57}}}
\]
\end{exercise}

\begin{exercise}
%% 11
Let $f(x)=\sqrt{x} e^{-3 x}+\frac{3 e^2}{x^7}$.
\[
\ddx f(x) = \answer{\frac{e^{-3 x}}{2 \sqrt{x}}-3 \sqrt{x} e^{-3 x} \ln (e)-\frac{21 e^2}{x^8}}
\]
\end{exercise}

\begin{exercise}
%% 12
Let $f(x)=-\frac{3 x}{\ln (x)-3 x^6}$.
\[
\ddx f(x) = \answer{-\frac{3 \left(15 x^6+\ln (x)-1\right)}{\left(\ln (x)-3 x^6\right)^2}}
\]
\end{exercise}

\begin{exercise}
%% 13
Let $f(x)=\sin (4 x) \left(-e^{\tan (x)}\right)$.
\[
\ddx f(x) = \answer{-e^{\tan (x)} \left(4 \cos (4 x)+\sin (4 x) \sec ^2(x)\right)}
\]
\end{exercise}

\begin{exercise}
%% 14
Let $f(x)=\sqrt{\sec (x)-\pi +3}$.
\[
\ddx f(x) = \answer{\frac{\tan (x) \sec (x)}{2 \sqrt{\sec (x)-\pi +3}}}
\]
\end{exercise}

\begin{exercise}
%% 15
Let $f(x)=\cos (\ln (x))$.
\[
\ddx f(x) = \answer{-\frac{\sin (\ln (x))}{x}}
\]
\end{exercise}

\begin{exercise}
%% 16
Let $f(x)=\ln (\cot (x))$.
\[
\ddx f(x) = \answer{-\csc (x) \sec (x)}
\]
\end{exercise}

\begin{exercise}
%% 1
Let $f(x)=-\frac{e^{-3 x} \sec (x)}{\pi }$.
\[
\ddx f(x) = \answer{-\frac{e^{-3 x} (\tan (x)-3) \sec (x)}{\pi }}
\]
\end{exercise}

\begin{exercise}
%% 2
Let $f(x)=-\frac{4}{x^5}+\sqrt{x}+e^{-3 x}+\frac{1}{\sqrt{x}}$.
\[
\ddx f(x) = \answer{\frac{1}{2} \left(\frac{x^{11/2}-x^{9/2}+40}{x^6}-6 e^{-3 x}\right)}
\]
\end{exercise}

\begin{exercise}
%% 3
Let $f(x)=\left(\frac{1}{x^5}-2\right) (x \cot (x)-4)$.
\[
\ddx f(x) = \answer{\frac{20-5 x \cot (x)}{x^6}+\left(\frac{1}{x^5}-2\right) \left(\cot (x)-x \csc ^2(x)\right)}
\]
\end{exercise}

\begin{exercise}
%% 4
Let $f(x)=5 x^{-\pi }+5^{e^2} x+5^x+\sec ^5(2)$.
\[
\ddx f(x) = \answer{-5 \pi  x^{-1-\pi }+5^x \ln (5)+5^{e^2}}
\]
\end{exercise}

\begin{exercise}
%% 5
Let $f(x)=\csc \left(\frac{x^4+2 x}{3-2 x^5}\right)$.
\[
\ddx f(x) = \answer{-\frac{2 \left(x^8+8 x^5+6 x^3+3\right) \cot \left(\frac{x \left(x^3+2\right)}{3-2 x^5}\right) \csc \left(\frac{x \left(x^3+2\right)}{3-2 x^5}\right)}{\left(3-2 x^5\right)^2}}
\]
\end{exercise}

\begin{exercise}
%% 6
Let $f(x)=\frac{\cos ^6(x)+\sec (3)}{\sqrt{x^5-2}+3}$.
\[
\ddx f(x) = \answer{-\frac{6 \sin (x) \cos ^5(x)}{\sqrt{x^5-2}+3}-\frac{5 x^4 \left(\cos ^6(x)+\sec (3)\right)}{2 \sqrt{x^5-2} \left(\sqrt{x^5-2}+3\right)^2}}
\]
\end{exercise}

\begin{exercise}
%% 7
Let $f(x)=x \ln (x \ln (x))$.
\[
\ddx f(x) = \answer{\ln (x \ln (x))+\frac{1}{\ln (x)}+1}
\]
\end{exercise}

\begin{exercise}
%% 8
Let $f(x)=\sqrt{3 x-\frac{3}{x^4}}$.
\[
\ddx f(x) = \answer{\frac{\frac{12}{x^5}+3}{2 \sqrt{3 x-\frac{3}{x^4}}}}
\]
\end{exercise}

\begin{exercise}
%% 9
Let $f(x)=4 x^{36}+e^x x+\ln ^5(3)$.
\[
\ddx f(x) = \answer{144 x^{35}+e^x (x+1)}
\]
\end{exercise}

\begin{exercise}
%% 10
Let $f(x)=\frac{823543}{x^{42}}-\frac{3}{\sqrt{x}}+\frac{\sin (x)}{x}$.
\[
\ddx f(x) = \answer{-\frac{\sin (x)}{x^2}+\frac{3 \left(x^{83/2}-23059204\right)}{2 x^{43}}+\frac{\cos (x)}{x}}
\]
\end{exercise}

\begin{exercise}
%% 11
Let $f(x)=\sqrt{x} e^{-3 x}-\frac{2 e}{x^6}$.
\[
\ddx f(x) = \answer{\frac{e^{-3 x} \left(24 e e^{3 x}-6 x^{15/2} \ln (e)+x^{13/2}\right)}{2 x^7}}
\]
\end{exercise}

\begin{exercise}
%% 12
Let $f(x)=-\frac{3 x}{2 x^6+\ln (x)}$.
\[
\ddx f(x) = \answer{\frac{30 x^6-3 \ln (x)+3}{\left(2 x^6+\ln (x)\right)^2}}
\]
\end{exercise}

\begin{exercise}
%% 13
Let $f(x)=\cos (3 x) e^{\tan (x)}$.
\[
\ddx f(x) = \answer{e^{\tan (x)} \left(\cos (3 x) \sec ^2(x)-3 \sin (3 x)\right)}
\]
\end{exercise}

\begin{exercise}
%% 14
Let $f(x)=\sqrt{\sec (x)+3+\ln (3)}$.
\[
\ddx f(x) = \answer{\frac{\tan (x) \sec (x)}{2 \sqrt{\sec (x)+3+\ln (3)}}}
\]
\end{exercise}

\begin{exercise}
%% 15
Let $f(x)=\csc (\ln (x))$.
\[
\ddx f(x) = \answer{-\frac{\cot (\ln (x)) \csc (\ln (x))}{x}}
\]
\end{exercise}

\begin{exercise}
%% 16
Let $f(x)=\ln (\sin (x))$.
\[
\ddx f(x) = \answer{\cot (x)}
\]
\end{exercise}

\begin{exercise}
%% 1
Let $f(x)=e^{-2 x-2} \csc (x)$.
\[
\ddx f(x) = \answer{-e^{-2 (x+1)} (\cot (x)+2) \csc (x)}
\]
\end{exercise}

\begin{exercise}
%% 2
Let $f(x)=\frac{2}{x^7}+\sqrt{x}+e^{-3 x}+\frac{1}{\sqrt{x}}$.
\[
\ddx f(x) = \answer{\frac{1}{2} \left(-\frac{1}{x^{3/2}}-\frac{28}{x^8}-6 e^{-3 x}+\frac{1}{\sqrt{x}}\right)}
\]
\end{exercise}

\begin{exercise}
%% 3
Let $f(x)=\left(x^5+3\right) (x \sec (x)-4)$.
\[
\ddx f(x) = \answer{\left(6 x^5+\left(x^5+3\right) x \tan (x)+3\right) \sec (x)-20 x^4}
\]
\end{exercise}

\begin{exercise}
%% 4
Let $f(x)=7 x^e+7^{e^2} x+7^x+\cos ^7(2)$.
\[
\ddx f(x) = \answer{7 e x^{e-1}+7^x \ln (7)+7^{e^2}}
\]
\end{exercise}

\begin{exercise}
%% 5
Let $f(x)=\cot \left(\frac{x^7-3 x}{-2 x^6-3}\right)$.
\[
\ddx f(x) = \answer{\frac{\left(2 x^{12}+51 x^6-9\right) \csc ^2\left(\frac{x \left(x^6-3\right)}{2 x^6+3}\right)}{\left(2 x^6+3\right)^2}}
\]
\end{exercise}

\begin{exercise}
%% 6
Let $f(x)=\frac{\sin ^7(x)+\sec (2)}{\sqrt{x^8+3}+4}$.
\[
\ddx f(x) = \answer{\frac{7 \left(\sqrt{x^8+3}+4\right) \sin ^6(x) \cos (x)-\frac{4 x^7 \left(\sin ^7(x)+\sec (2)\right)}{\sqrt{x^8+3}}}{\left(\sqrt{x^8+3}+4\right)^2}}
\]
\end{exercise}

\begin{exercise}
%% 7
Let $f(x)=-\infty$.
\[
\ddx f(x) = \answer{0}
\]
\end{exercise}

\begin{exercise}
%% 8
Let $f(x)=\sqrt{2 x-\frac{3}{x^6}}$.
\[
\ddx f(x) = \answer{\frac{x^7+9}{x^7 \sqrt{2 x-\frac{3}{x^6}}}}
\]
\end{exercise}

\begin{exercise}
%% 9
Let $f(x)=2 x^{42}+e^x x+e^{10}$.
\[
\ddx f(x) = \answer{84 x^{41}+e^x (x+1)}
\]
\end{exercise}

\begin{exercise}
%% 10
Let $f(x)=\frac{823543}{x^{49}}+\frac{4}{\sqrt{x}}+\frac{\cos (x)}{x}$.
\[
\ddx f(x) = \answer{-\frac{2 x^{97/2}+x^{49} \sin (x)+x^{48} \cos (x)+40353607}{x^{50}}}
\]
\end{exercise}

\begin{exercise}
%% 11
Let $f(x)=\sqrt{x} e^{-4 x}+\frac{2 \pi }{x^8}$.
\[
\ddx f(x) = \answer{\frac{e^{-4 x}}{2 \sqrt{x}}-4 \sqrt{x} e^{-4 x} \ln (e)-\frac{16 \pi }{x^9}}
\]
\end{exercise}

\begin{exercise}
%% 12
Let $f(x)=\frac{4 x}{4 x^8+\ln (x)}$.
\[
\ddx f(x) = \answer{\frac{4 \left(-28 x^8+\ln (x)-1\right)}{\left(4 x^8+\ln (x)\right)^2}}
\]
\end{exercise}

\begin{exercise}
%% 13
Let $f(x)=\sin (3 x) e^{\tan (x)}$.
\[
\ddx f(x) = \answer{e^{\tan (x)} \left(3 \cos (3 x)+\sin (3 x) \sec ^2(x)\right)}
\]
\end{exercise}

\begin{exercise}
%% 14
Let $f(x)=\sqrt{\csc (x)+3+\ln (3)}$.
\[
\ddx f(x) = \answer{-\frac{\cot (x) \csc (x)}{2 \sqrt{\csc (x)+3+\ln (3)}}}
\]
\end{exercise}

\begin{exercise}
%% 15
Let $f(x)=\cot (\ln (x))$.
\[
\ddx f(x) = \answer{-\frac{\csc ^2(\ln (x))}{x}}
\]
\end{exercise}

\begin{exercise}
%% 16
Let $f(x)=\ln (\ln (x))$.
\[
\ddx f(x) = \answer{\frac{1}{x \ln (x)}}
\]
\end{exercise}

\begin{exercise}
%% 1
Let $f(x)=e^{-3 x-1} \cot (x)$.
\[
\ddx f(x) = \answer{-e^{-3 x-1} \left(3 \cot (x)+\csc ^2(x)\right)}
\]
\end{exercise}

\begin{exercise}
%% 2
Let $f(x)=-4 x^6+\sqrt{x}+e^{-4 x}+\frac{1}{\sqrt[5]{x}}$.
\[
\ddx f(x) = \answer{-24 x^5-4 e^{-4 x}+\frac{1}{2 \sqrt{x}}-\frac{1}{5 \sqrt[5]{x} x}}
\]
\end{exercise}

\begin{exercise}
%% 3
Let $f(x)=\left(\frac{1}{x^8}+4\right) (x \sin (x)+4)$.
\[
\ddx f(x) = \answer{\left(\frac{1}{x^8}+4\right) (\sin (x)+x \cos (x))-\frac{8 (x \sin (x)+4)}{x^9}}
\]
\end{exercise}

\begin{exercise}
%% 4
Let $f(x)=6 x^{\ln (5)}+6^x+x 6^{\sec (2)}+e^6$.
\[
\ddx f(x) = \answer{6 \ln (5) x^{\ln (5)-1}+6^x \ln (6)+6^{\sec (2)}}
\]
\end{exercise}

\begin{exercise}
%% 5
Let $f(x)=\sec \left(\frac{x^5-4 x}{4 x^6-2}\right)$.
\[
\ddx f(x) = \answer{-\frac{\left(2 x^{10}-40 x^6+5 x^4-4\right) \tan \left(\frac{x \left(x^4-4\right)}{4 x^6-2}\right) \sec \left(\frac{x \left(x^4-4\right)}{4 x^6-2}\right)}{2 \left(1-2 x^6\right)^2}}
\]
\end{exercise}

\begin{exercise}
%% 6
Let $f(x)=\frac{\cos ^7(x)+e}{\sqrt{x^7+2}-2}$.
\[
\ddx f(x) = \answer{\frac{7 \left(-2 \left(\sqrt{x^7+2}-2\right) \sin (x) \cos ^6(x)-\frac{x^6 \left(\cos ^7(x)+e\right)}{\sqrt{x^7+2}}\right)}{2 \left(\sqrt{x^7+2}-2\right)^2}}
\]
\end{exercise}

\begin{exercise}
%% 7
Let $f(x)=x \ln (x \ln (x))$.
\[
\ddx f(x) = \answer{\ln (x \ln (x))+\frac{1}{\ln (x)}+1}
\]
\end{exercise}

\begin{exercise}
%% 8
Let $f(x)=\sqrt{-\frac{3}{x^8}-3 x}$.
\[
\ddx f(x) = \answer{\frac{\frac{24}{x^9}-3}{2 \sqrt{-\frac{3}{x^8}-3 x}}}
\]
\end{exercise}

\begin{exercise}
%% 9
Let $f(x)=4 x^{20}+e^x x+e^{14}$.
\[
\ddx f(x) = \answer{80 x^{19}+e^x (x+1)}
\]
\end{exercise}

\begin{exercise}
%% 10
Let $f(x)=\frac{5764801}{x^{32}}-\frac{2}{\sqrt{x}}+\frac{\tan (x)}{x}$.
\[
\ddx f(x) = \answer{\frac{x^{63/2}+x^{32} \sec ^2(x)-x^{31} \tan (x)-184473632}{x^{33}}}
\]
\end{exercise}

\begin{exercise}
%% 11
Let $f(x)=\sqrt{x} e^{4 x}-\frac{4 \pi }{x^6}$.
\[
\ddx f(x) = \answer{\frac{e^{4 x}}{2 \sqrt{x}}+4 \sqrt{x} e^{4 x} \ln (e)+\frac{24 \pi }{x^7}}
\]
\end{exercise}

\begin{exercise}
%% 12
Let $f(x)=\frac{3 x}{3 x^6+\ln (x)}$.
\[
\ddx f(x) = \answer{\frac{-45 x^6+3 \ln (x)-3}{\left(3 x^6+\ln (x)\right)^2}}
\]
\end{exercise}

\begin{exercise}
%% 13
Let $f(x)=\cos (4 x) e^{\csc (x)}$.
\[
\ddx f(x) = \answer{-e^{\csc (x)} (4 \sin (4 x)+\cos (4 x) \cot (x) \csc (x))}
\]
\end{exercise}

\begin{exercise}
%% 14
Let $f(x)=\sqrt{\cot (x)+3+\sec (3)}$.
\[
\ddx f(x) = \answer{-\frac{\csc ^2(x)}{2 \sqrt{\cot (x)+3+\sec (3)}}}
\]
\end{exercise}

\begin{exercise}
%% 15
Let $f(x)=\tan (\ln (x))$.
\[
\ddx f(x) = \answer{\frac{\sec ^2(\ln (x))}{x}}
\]
\end{exercise}

\begin{exercise}
%% 16
Let $f(x)=\ln (\cot (x))$.
\[
\ddx f(x) = \answer{-\csc (x) \sec (x)}
\]
\end{exercise}

\begin{exercise}
%% 1
Let $f(x)=e^{-3 x-2} \cos (x)$.
\[
\ddx f(x) = \answer{-e^{-3 x-2} (\sin (x)+3 \cos (x))}
\]
\end{exercise}

\begin{exercise}
%% 2
Let $f(x)=-\frac{2}{x^7}+\sqrt{x}+e^{-3 x}+\frac{1}{\sqrt[3]{x}}$.
\[
\ddx f(x) = \answer{\frac{x^{15/2}+28}{2 x^8}-3 e^{-3 x}-\frac{1}{3 x \sqrt[3]{x}}}
\]
\end{exercise}

\begin{exercise}
%% 3
Let $f(x)=\left(\frac{1}{x^7}-4\right) (x \sec (x)-2)$.
\[
\ddx f(x) = \answer{\frac{14-7 x \sec (x)}{x^8}+\left(\frac{1}{x^7}-4\right) (x \tan (x)+1) \sec (x)}
\]
\end{exercise}

\begin{exercise}
%% 4
Let $f(x)=7 x^{-e}+7^{-\pi } x+7^x+\sec ^7(2)$.
\[
\ddx f(x) = \answer{-7 e x^{-1-e}+7^x \ln (7)+7^{-\pi }}
\]
\end{exercise}

\begin{exercise}
%% 5
Let $f(x)=\sin \left(\frac{x^8-3 x}{4 x^4+4}\right)$.
\[
\ddx f(x) = \answer{\frac{\left(4 x^{11}+8 x^7+9 x^4-3\right) \cos \left(\frac{x \left(x^7-3\right)}{4 \left(x^4+1\right)}\right)}{4 \left(x^4+1\right)^2}}
\]
\end{exercise}

\begin{exercise}
%% 6
Let $f(x)=\frac{\cot ^4(x)+e^2}{\sqrt{x^4+2}-4}$.
\[
\ddx f(x) = \answer{\frac{2 \left(-2 \left(\sqrt{x^4+2}-4\right) \cot ^3(x) \csc ^2(x)-\frac{x^3 \left(\cot ^4(x)+e^2\right)}{\sqrt{x^4+2}}\right)}{\left(\sqrt{x^4+2}-4\right)^2}}
\]
\end{exercise}

\begin{exercise}
%% 7
Let $f(x)=x \ln (x \ln (x))$.
\[
\ddx f(x) = \answer{\ln (x \ln (x))+\frac{1}{\ln (x)}+1}
\]
\end{exercise}

\begin{exercise}
%% 8
Let $f(x)=\sqrt{-\frac{3}{x^6}-3 x}$.
\[
\ddx f(x) = \answer{\frac{\frac{18}{x^7}-3}{2 \sqrt{-\frac{3}{x^6}-3 x}}}
\]
\end{exercise}

\begin{exercise}
%% 9
Let $f(x)=2 x^{36}+e^x x+\pi ^8$.
\[
\ddx f(x) = \answer{72 x^{35}+e^x (x+1)}
\]
\end{exercise}

\begin{exercise}
%% 10
Let $f(x)=\frac{117649}{x^{48}}+\frac{3}{\sqrt{x}}+\frac{\tan (x)}{x}$.
\[
\ddx f(x) = \answer{-\frac{3}{2 x^{3/2}}-\frac{5647152}{x^{49}}-\frac{\tan (x)}{x^2}+\frac{\sec ^2(x)}{x}}
\]
\end{exercise}

\begin{exercise}
%% 11
Let $f(x)=\sqrt{x} e^{4 x}-\frac{4 \pi }{x^8}$.
\[
\ddx f(x) = \answer{\frac{e^{4 x}}{2 \sqrt{x}}+4 \sqrt{x} e^{4 x} \ln (e)+\frac{32 \pi }{x^9}}
\]
\end{exercise}

\begin{exercise}
%% 12
Let $f(x)=-\frac{2 x}{\ln (x)-2 x^4}$.
\[
\ddx f(x) = \answer{-\frac{2 \left(6 x^4+\ln (x)-1\right)}{\left(\ln (x)-2 x^4\right)^2}}
\]
\end{exercise}

\begin{exercise}
%% 13
Let $f(x)=\cot (2 x) \left(-e^{\csc (x)}\right)$.
\[
\ddx f(x) = \answer{e^{\csc (x)} \left(2 \csc ^2(2 x)+\cot (x) \cot (2 x) \csc (x)\right)}
\]
\end{exercise}

\begin{exercise}
%% 14
Let $f(x)=\sqrt{\cos (x)-e+3}$.
\[
\ddx f(x) = \answer{-\frac{\sin (x)}{2 \sqrt{\cos (x)-e+3}}}
\]
\end{exercise}

\begin{exercise}
%% 15
Let $f(x)=\cot (\ln (x))$.
\[
\ddx f(x) = \answer{-\frac{\csc ^2(\ln (x))}{x}}
\]
\end{exercise}

\begin{exercise}
%% 16
Let $f(x)=\ln (\tan (x))$.
\[
\ddx f(x) = \answer{\csc (x) \sec (x)}
\]
\end{exercise}

\begin{exercise}
%% 1
Let $f(x)=-e^{4 x-1} \sec (x)$.
\[
\ddx f(x) = \answer{-e^{4 x-1} (\tan (x)+4) \sec (x)}
\]
\end{exercise}

\begin{exercise}
%% 2
Let $f(x)=3 x^5+\sqrt{x}+e^{-3 x}+\frac{1}{\sqrt{x}}$.
\[
\ddx f(x) = \answer{\frac{1}{2} \left(\frac{30 x^{11/2}+x-1}{x^{3/2}}-6 e^{-3 x}\right)}
\]
\end{exercise}

\begin{exercise}
%% 3
Let $f(x)=\left(x^5-4\right) (x \cot (x)-3)$.
\[
\ddx f(x) = \answer{\left(x^5-4\right) \left(\cot (x)-x \csc ^2(x)\right)+5 x^4 (x \cot (x)-3)}
\]
\end{exercise}

\begin{exercise}
%% 4
Let $f(x)=7 x^{-e}+7^x+x 7^{\cos (3)}+e^7$.
\[
\ddx f(x) = \answer{-7 e x^{-1-e}+7^x \ln (7)+7^{\cos (3)}}
\]
\end{exercise}

\begin{exercise}
%% 5
Let $f(x)=\csc \left(\frac{x^5+2 x}{-2 x^4-4}\right)$.
\[
\ddx f(x) = \answer{\frac{1}{4} \sin (x) \csc ^3\left(\frac{x}{2}\right)}
\]
\end{exercise}

\begin{exercise}
%% 6
Let $f(x)=\frac{\cos ^4(x)+\ln (3)}{\sqrt{x^6+3}+3}$.
\[
\ddx f(x) = \answer{\frac{-4 \left(\sqrt{x^6+3}+3\right) \sin (x) \cos ^3(x)-\frac{3 x^5 \left(\cos ^4(x)+\ln (3)\right)}{\sqrt{x^6+3}}}{\left(\sqrt{x^6+3}+3\right)^2}}
\]
\end{exercise}

\begin{exercise}
%% 7
Let $f(x)=x \ln (x \ln (x))$.
\[
\ddx f(x) = \answer{\ln (x \ln (x))+\frac{1}{\ln (x)}+1}
\]
\end{exercise}

\begin{exercise}
%% 8
Let $f(x)=\sqrt{-\frac{3}{x^7}-4 x}$.
\[
\ddx f(x) = \answer{\frac{\frac{21}{x^8}-4}{2 \sqrt{-\frac{3}{x^7}-4 x}}}
\]
\end{exercise}

\begin{exercise}
%% 9
Let $f(x)=-4 x^{36}+e^x x+\pi ^6$.
\[
\ddx f(x) = \answer{e^x (x+1)-144 x^{35}}
\]
\end{exercise}

\begin{exercise}
%% 10
Let $f(x)=\frac{16807}{x^{20}}+\frac{2}{\sqrt{x}}+\frac{\tan (x)}{x}$.
\[
\ddx f(x) = \answer{-\frac{x^{39/2}+x^{20} \left(-\sec ^2(x)\right)+x^{19} \tan (x)+336140}{x^{21}}}
\]
\end{exercise}

\begin{exercise}
%% 11
Let $f(x)=\sqrt{x} e^{4 x}-\frac{2 e}{x^7}$.
\[
\ddx f(x) = \answer{\frac{e^{4 x}}{2 \sqrt{x}}+4 \sqrt{x} e^{4 x} \ln (e)+\frac{14 e}{x^8}}
\]
\end{exercise}

\begin{exercise}
%% 12
Let $f(x)=-\frac{4 x}{\ln (x)-3 x^5}$.
\[
\ddx f(x) = \answer{-\frac{4 \left(12 x^5+\ln (x)-1\right)}{\left(\ln (x)-3 x^5\right)^2}}
\]
\end{exercise}

\begin{exercise}
%% 13
Let $f(x)=e^{\sin (x)} \cos (3 x)$.
\[
\ddx f(x) = \answer{e^{\sin (x)} (\cos (x) \cos (3 x)-3 \sin (3 x))}
\]
\end{exercise}

\begin{exercise}
%% 14
Let $f(x)=\sqrt{\sec (x)-e+3}$.
\[
\ddx f(x) = \answer{\frac{\tan (x) \sec (x)}{2 \sqrt{\sec (x)-e+3}}}
\]
\end{exercise}

\begin{exercise}
%% 15
Let $f(x)=\sin (\ln (x))$.
\[
\ddx f(x) = \answer{\frac{\cos (\ln (x))}{x}}
\]
\end{exercise}

\begin{exercise}
%% 16
Let $f(x)=\ln (\cot (x))$.
\[
\ddx f(x) = \answer{-\csc (x) \sec (x)}
\]
\end{exercise}


  
\end{shuffle}


\end{document}
