\documentclass{ximera}

\input{../../preamble.tex}

\author{Jim Talamo}
\license{Creative Commons 3.0 By-NC}


\outcome{Review integration techniques}


\begin{document}
\begin{exercise}
Consider the initial value problem below:

\[
(x^2+1) \dd[y]{x} = 4xe^{2y}  , \qquad y(0)=0
\]

<IMAGE TO BE INCLUDED ON AN UPDATE - PLEASE LOOK AT THE SAMPLE PROBLEMS FROM CLASS>
%%%%%MAKE A MAPLE PICTURE%%%%%%%%%
%The direction field for the differential equation is:
%
%\begin{image}
%{\def\length{sqrt(1+((4*x*exp(2*y))/(x^2+1))^2)}
%\begin{tikzpicture}
%  \begin{axis}[
%      xmin=-1, xmax=1,ymin=-1,ymax=1,domain=-1:1,view={0}{90},
%      axis lines =center, xlabel=$x$, ylabel=$y$,
%      every axis y label/.style={at=(current axis.above origin),anchor=south},
%      every axis x label/.style={at=(current axis.right of origin),anchor=west},
%      axis on top,
%    ] 
%    \addplot3 [penColor, quiver={u={1/\length}, v={(4*x*exp(2*y))/(x^2+1)/(\length)},scale arrows=.2},samples=10] {0};
%]  \end{axis}
%\end{tikzpicture}}
%\end{image}
%



The solution of the initial value problem is $y(x) = \answer{-\frac{1}{2}\ln(1-4 \ln(x^2+1))  }$.

\begin{hint}
The differentials $\d y$ and $\d x$ are related by:

\[
\left(\answer{e^{-2y}} \right) \d y = \left(\answer{ \frac{4x}{x^2+1} } \right) \d x
\]

\begin{question}
We can now integrate both sides.

To integrate the righthand side:

\begin{multipleChoice}
\choice{Use the integration formula involving an inverse tangent.}
\choice[correct]{Use a $u$-substitution}
\choice{Use integration by parts}
\choice{Use partial fraction decomposition}
\end{multipleChoice}

Carrying out the integration of both sides gives:

\begin{align*}
\answer{-\frac{1}{2}e^{-2y}} &= \answer{2 \ln(x^2+1)} +C\\
\end{align*}

Using the initial condition, we find $C=\answer{-\frac{1}{2}}$.

\begin{question}

We thus have:

\begin{align*}
-\frac{1}{2}e^{-2y} &= 2 \ln(x^2+1) -\frac{1}{2} \\
e^{-2y} &= \answer{-4 \ln(x^2+1)+1} \\
y&= \answer{-\frac{1}{2}\ln(-4 \ln(x^2+1)+1)}
\end{align*}

\end{question}
\end{question}
 \end{hint}
 
\begin{exercise}
Find all $x$-values for which the solution is defined.

The solution is defined for $\answer{-\sqrt{e^{1/4}-1}} < x <  \answer{\sqrt{e^{1/4}-1}}$.

\begin{hint}
The solution $y= -\frac{1}{2}\ln(-4 \ln(x^2+1)+1)$ will be defined whenever $-4 \ln(x^2+1)+1 >0$.  From this we find:

\begin{align*}
\ln(x^2+1) < \frac{1}{4} \\
x^2+1 < \answer{e^{1/4}} \\
x^2 < \answer{e^{1/4}-1} \\
\end{align*}

This means that both  $x>  \answer{-\sqrt{e^{1/4}-1}}$ and $x<  \answer{\sqrt{e^{1/4}-1}}$.
\end{hint}
\end{exercise}
 
\end{exercise}
\end{document}
