\documentclass{ximera}

\input{../../preamble.tex}

\author{Jim Talamo}
\license{Creative Commons 3.0 By-bC}


\outcome{}


\begin{document}
\begin{exercise}
Consider the power series $\sum_{k=0}^{\infty} \frac{2^k}{5k-1}(x-1)^{k}$.

We want to determine the interval of convergence for this power series. 

First, we use the Ratio Test to determine the interval of convergence. 

We need to determine the limit $\lim_{k \to \infty} \left| \frac{a_{k+1}}{a_k}\right|$. 

We calculate $a_{k+1}=\answer{\frac{2^{k+1}}{5k+4}(x-1)^{k+1}}$ and $a_k=\answer{ \frac{2^k}{5k-1}(x-1)^k}$. 

\begin{exercise}

Simplifying the ratio $\left|\frac{a_{k+1}}{a_k}\right|$ gives us $\left|\frac{a_{k+1}}{a_k}\right|=\answer{\frac{2(5k-1)}{5k-4} |x-1|}$.


\begin{exercise}

We calculate the limit

\[
\lim_{k \to \infty}  \frac{2(5k-1)}{5k-4} |x-1| =\answer{ 2|x-1|}
\]

\begin{exercise}

Recall the Ratio Test tells us that a series $\sum^{\infty}_{k=1} a_k$ converges if $L <1$ where $L=\lim_{k \to \infty}\left| \frac{a_{k+1}}{a_k}\right|$. 

Thus in order to determine the set of $x$ for which our power series converges, we need to determine those $x$ which satisfy 
the inequality $2|x-1| <1$. 

Rewriting this inequality we obtain $|x-1|< \answer{\frac{1}{2}}$. 

Thus the  power series $\sum_{k=0}^{\infty} \frac{2^k}{5k-1}(x-1)^{k}$ has radius of convergence $\answer{\frac{1}{2}}$.

\begin{exercise}

By definition 
\[
|x-1|=\begin{cases}
  x-1 &\text{if $x-1\geq 0$} \\
 -(x-1) &\text{if $x-1 < 0$}
\end{cases}
\]

Thus we can rewrite $|x-1| < \frac{1}{2}$ as $\answer{\frac{-1}{2}} < x-1 < \answer{\frac{1}{2}}$ 


The radius of convergence for the power series is $\answer{\frac{1}{2}}$.

The lefthand endpoint of the interval of convergence is $x=\answer{\frac{1}{2}}$ and the righthand endpoint is $x= \answer{\frac{3}{2}}$.


\begin{exercise} 
Now we need to determine if our power series converges at the endpoints $x=\frac{1}{2}$ and $x=\frac{3}{2}$. 

First we test convergence at $x=\frac{1}{2}$. 

We plug $x=\frac{1}{2}$ into $\sum_{k=0}^{\infty} \frac{2^k}{5k-1}(x-1)^{k}$ to get

\[
\sum^{\infty}_{k=0} \answer{\frac{(-1)^k}{5k-1}}
\]


This series \wordChoice{\choice[correct]{converges}\choice{diverges}} 

\begin{multipleChoice}
\choice[correct]{converges}
\choice{diverges}
\end{multipleChoice}

Now we plug $x=\frac{3}{2}$ into $\sum_{k=0}^{\infty} \frac{2^k}{5k-1}(x-1)^{k}$ to get

\[
\sum^{\infty}_{k=0} \frac{1}{5k-1}
\]


This series \wordChoice{\choice{converges}\choice[correct]{diverges}}. 




\begin{exercise}
The interval of convergence of the power series $\sum_{k=0}^{\infty} \frac{2^k}{5k-1}(x-1)^{k}$ is:
\begin{multipleChoice}
\choice{$\left(\frac{1}{2},\frac{3}{2}\right)$}
\choice{$\left(\frac{1}{2},\frac{3}{2}\right]$}
\choice[correct]{$\left[\frac{1}{2},\frac{3}{2}\right)$}
\choice{$\left[\frac{1}{2},\frac{3}{2}\right]$}
\end{multipleChoice}







\end{exercise}

\end{exercise}
\end{exercise}
\end{exercise}
\end{exercise}
\end{exercise}
\end{exercise}
\end{document}
